AbstractDomain.fst
@@ -1,0 +1,56 @@
+module AbstractDomain
+
+open DefaultValue
+open FStar.Tactics.Typeclasses
+
+class hasAbstractDomain a = {
+  union : a -> a -> a;
+  inter : a -> a -> a;
+  bottom: a;
+  top   : a;
+  widen : a -> a -> a;
+  assign: string -> a -> a;
+  aeq : a -> a -> bool;
+}
+let mkAbstractDomain union inter bottom top widen assign aeq
+    = {
+        union = union
+      ; inter = inter
+      ; bottom = bottom
+      ; top = top
+      ; widen = widen
+      ; assign = assign
+      ; aeq = aeq
+    }
+
+class hasAbstractOperators a = {
+    abstract_domain:  hasAbstractDomain a
+  ; default_value:    hasDefaultValue a
+  ; a_op_unary_minus: a -> a
+  ; a_op_plus:        a -> a -> a
+  ; a_op_minus:       a -> a -> a
+  ; a_op_times:       a -> a -> a
+}
+let mkAbstractOperators #a [| hasAbstractDomain a |] [| hasDefaultValue a |]
+  a_op_unary_minus a_op_plus a_op_minus a_op_times
+  = {
+    abstract_domain  = solve
+  ; default_value    = solve
+  ; a_op_unary_minus = a_op_unary_minus
+  ; a_op_plus        = a_op_plus
+  ; a_op_minus       = a_op_minus
+  ; a_op_times       = a_op_times
+  }
+
+let backward_aop_le0         #a [| hasAbstractOperators a |] [| hasAbstractDomain a |] (x r  :a) (lessThanZero:a)
+    = x `inter` lessThanZero
+let backward_aop_unary_minus #a [| hasAbstractOperators a |] [| hasAbstractDomain a |] (x r  :a)
+    = x `inter` (a_op_unary_minus r)
+let backward_aop_plus        #a [| hasAbstractOperators a |] [| hasAbstractDomain a |] (x y r:a)
+    = (x `inter` (r `a_op_minus` y), y `inter` (r `a_op_minus` r)) 
+let backward_aop_minus       #a [| hasAbstractOperators a |] [| hasAbstractDomain a |] (x y r:a)
+    = (x `inter` (r `a_op_plus` y), y `inter` (x `a_op_minus` r)) 
+// let backward_aop_mul #a [| hasAbstractOperators a |] [| hasAbstractDomain a |] (x y r:a)
+//     = (x `inter` (r `a_op` y), y `inter` (r `a_op_minus` r))
+
+// let backward_aop_lt #a [| hasAbstractOperators a |] = 
