CSetPO.fst
@@ -1,0 +1,17 @@
+module CSetPO
+
+open CSet
+open PartialOrder
+
+open FStar.Tactics
+open FStar.Tactics.Typeclasses
+
+instance csetLPO #c : hasLPartialOrder (CSet.set c) = {
+    l_po_cmp = CSet.equal;
+    l_po = let h = (fun (a b: CSet.set c) -> true == CSet.subset a b) in admitP (isPartialOrderL CSet.equal h); h
+}
+
+instance gsetLPO #c : hasLPartialOrder (GSet.set c) = {
+    l_po_cmp = GSet.equal;
+    l_po = GSet.subset
+}
