GaloisConnection.fst
@@ -1,0 +1,34 @@
+module GaloisConnection
+
+open FStar.Tactics.Typeclasses
+open PartialOrder
+module CSet = CSet
+open FStar.GSet
+open CSetPO
+
+class hasGaloisConnection (c:eqtype) a = {
+     c_po  : hasPartialOrder c
+   ; a_po  : hasPartialOrder a
+   ; gamma : (f:(a -> set c){ isMonotonic f })
+   ; alpha : (f:(CSet.set c -> a){ isMonotonic f })
+   ; galois_wf : (sa:a) -> (sc:CSet.set c) ->
+		 Lemma (CSet.cset_to_set sc `l_po` (gamma sa) /\ sa `l_po` (alpha sc))
+   ; alpha': c -> a
+}
+
+let mkGaloisConnection (#c:eqtype) #a
+			     [| hasPartialOrder c |]
+			     [| hasPartialOrder a |]
+			     (gamma:(a -> set c){ isMonotonic gamma })
+			     (alpha:(CSet.set c -> a){ isMonotonic alpha })
+			     (galois_wf : (sa:a) -> (sc:CSet.set c) -> 
+					Lemma (CSet.cset_to_set sc `l_po` (gamma sa) /\ sa `l_po` (alpha sc))
+			     )
+  = {
+	c_po      = solve
+      ; a_po      = solve
+      ; gamma     = gamma
+      ; alpha     = alpha
+      ; galois_wf = galois_wf
+      ; alpha'    = (fun c -> alpha (CSet.singleton c))
+    }
