PartialOrder.fst
@@ -1,0 +1,33 @@
+module PartialOrder
+open FStar.Tactics.Typeclasses
+
+let isPartialOrder #a (f:(a -> a -> bool)) =
+    (forall a    . f a a)
+  /\ (forall a b  . f a b /\ f b a ==> a == b)
+  /\ (forall a b c. f a b /\ f b c ==> f a c)
+
+class hasPartialOrder a = {
+   po : (f:(a -> a -> bool){isPartialOrder f})
+}
+
+let isPartialOrderL #a (cmp:a->a->Type0) (f:(a -> a -> Type0)) =
+    (forall a    . f a a)
+  /\ (forall a b  . f a b /\ f b a ==> cmp a b)
+  /\ (forall a b c. f a b /\ f b c ==> f a c)
+  
+class hasLPartialOrder (a:Type) = {
+  l_po_cmp : a -> a -> Type;
+  l_po : (f:(a -> a -> Type){isPartialOrderL l_po_cmp f})
+}
+
+(* generic instance *)
+instance derivedLPO (someInstance : hasPartialOrder 'a) : hasLPartialOrder 'a = {
+  l_po_cmp = (fun x y -> x == y);
+  l_po = fun x y -> po x y == true
+}
+(* int instance *)
+instance _ : hasPartialOrder int = { po = fun a b -> a <= b } 
+
+(* isMonotonic *)
+let isMonotonic #a #b [| hasLPartialOrder a |] [| hasLPartialOrder b |] (f:(a -> b)) =
+  forall a b. a `l_po` b ==> f(a) `l_po` f(b)
