StaticAnalyser.fst
@@ -1,0 +1,88 @@
+module StaticAnalyser
+
+open FStar.GSet
+module CS = CSet
+open FStar.Tactics
+open FStar.Tactics.Typeclasses
+
+open PartialOrder
+open GaloisConnection
+open DefaultValue
+open ToyLanguageDef
+open EnumerableMap
+open AbstractDomain
+open ZeroOrLess
+
+let rec static_analysis_aexp #a [| hasGaloisConnection int a |] [| hasAbstractOperators a |]
+                    (st:enumerableMap a)
+                    (exp:lAExp)
+                    : a
+  = let rec h (exp:lAExp): a = 
+         match exp with
+       | LAExpLitt n       -> alpha' n
+       | LAExpVar  varName -> em_get st varName
+       | LAExpPlus a b     -> (h a) `a_op_plus` (h b)
+       | LAExpMinus a b    -> (h a) `a_op_minus` (h b)
+       | LAExpMult a b    ->  (h a) `a_op_times` (h b)
+    in h exp
+
+let rec backward_analysis_aexp #a [| hasGaloisConnection int a |] [| hasAbstractOperators a |]
+                                  [| hasAbstractDomain a |]
+                    (st:enumerableMap a)
+                    (exp:lAExp)
+                    (aim:a)
+                    : Tot (enumerableMap a) (decreases exp)
+= let f exp = static_analysis_aexp st exp in
+  match exp with
+  | LAExpLitt n       -> st //(alpha' n) `inter` aim
+  | LAExpVar  varName -> em_set st varName aim//(st varName) ``
+  | LAExpPlus e1 e2   -> let (aim1, aim2):(tuple2 a a) = backward_aop_plus (f e1) (f e2) aim in (* e1 + e1 should fit in aim *)
+                        let st' = backward_analysis_aexp st e1 aim1 in
+                        backward_analysis_aexp st' e2 aim2
+  | LAExpMinus e1 e2  -> let (aim1, aim2):(tuple2 a a) = backward_aop_minus (f e1) (f e2) aim in (* e1 + e1 should fit in aim *)
+                        let st' = backward_analysis_aexp st e1 aim1 in
+                        backward_analysis_aexp st' e2 aim2
+  | LAExpMult a b    ->  st (*todo*)//(h a) `a_op_times` (h b)
+
+let rec analyse_bexp #a [| hasAbstractOperators a |] [| hasAbstractDomain a |] [| hasGaloisConnection int a |] [| hasZeroOrLess a |]
+                     (st:enumerableMap a)
+                     (exp:lBExp): Tot (enumerableMap a)
+                                  (decreases %[bexp_count_not exp; exp])
+  = match exp with
+  | LBExpLitt b -> if b then st (* supposing true doesn't bring anything new *)
+                       else {_em_data = (fun _ -> bottom); _em_keys = st._em_keys} (* variables should all be bottom *)
+  | LBExpNot (LBExpEq a b) -> backward_analysis_aexp st (a -. b) (alpha' 0)
+  | LBExpNot  b -> let rec apply_not (e:lBExp): (r:lBExp{bexp_count_not e >= bexp_count_not r}) = (match e with
+                          | LBExpNot e1    -> e1
+                          | LBExpAnd e1 e2 -> LBExpOr  (apply_not e1) (apply_not e2)
+                          | LBExpOr  e1 e2 -> LBExpAnd (apply_not e1) (apply_not e2)
+                          | LBExpLe  e1 e2 -> (e2 <=. e1) &&. (!. (e1 ==. e2))
+                          | LBExpEq  e1 e2 -> LBExpNot e
+                          | LBExpLitt   _  -> e
+                          ) in 
+                            let nexp = apply_not b in
+                               analyse_bexp st nexp
+  | LBExpAnd  a b -> em_combine (analyse_bexp st a) (analyse_bexp st b) inter
+  | LBExpOr   a b -> em_combine (analyse_bexp st a) (analyse_bexp st b) union
+  | LBExpEq   a b -> backward_analysis_aexp st (a -. b) (alpha' 0)//lessThanZero
+  | LBExpLe   a b -> backward_analysis_aexp st (a -. b) zeroOrLess
+
+let rec static_analysis_instr #a [| hasAbstractOperators a |] [| hasAbstractDomain a |] [| hasGaloisConnection int a |] [| hasZeroOrLess a |]
+                    (st:enumerableMap a)
+                    (instr:lInstr)
+                    : Tot (enumerableMap a) (decreases instr)
+  = let f = static_analysis_instr in
+    match instr with
+  | LInstrAssign name v -> em_set st name (static_analysis_aexp st v)
+  | LInstrSkip          -> st
+  | LInstrSeq b1 b2     -> static_analysis_instr (f st b1) b2 
+  | LInstrIf c b1 b2    -> let r1 = f (analyse_bexp st     c ) b1 in
+                          let r2 = f (analyse_bexp st (!. c)) b2 in
+                          em_combine r1 r2 union
+  | LInstrWhile cond b1 -> let apply_cond st = analyse_bexp st cond in
+                          let rec lookForFixPoint current_st (stop: nat): Tot (enumerableMap a) = if stop=0 then current_st else
+                              let new_st  = static_analysis_instr (apply_cond current_st) b1 in
+                              let widened = em_combine new_st (apply_cond (em_combine current_st new_st widen)) union in 
+                                if   em_equal aeq current_st widened then widened
+                                else lookForFixPoint (admitP (%[widened] << %[current_st]); widened) (stop - 1) in
+                          em_combine (analyse_bexp st (!. cond)) (lookForFixPoint st 4) union
