ToString.fst
@@ -1,0 +1,10 @@
+module ToString
+
+open FStar.Tactics.Typeclasses
+open FStar.String
+
+class hasToString t = {
+  toString: t -> string
+}
+
+let join sep l = List.Tot.Base.fold_right (fun a b -> (if a = "" then sep else "") `strcat` (a `strcat` b)) l ""
