ToyLanguageDef.fst
@@ -1,0 +1,62 @@
+module ToyLanguageDef
+open FStar.Tactics.Typeclasses
+
+type lAExp =
+  | LAExpLitt : int -> lAExp
+  | LAExpVar  : string -> lAExp
+  | LAExpPlus : lAExp -> lAExp -> lAExp 
+  | LAExpMinus: lAExp -> lAExp -> lAExp 
+  | LAExpMult : lAExp -> lAExp -> lAExp
+
+let ( +. ) = LAExpPlus
+let ( -. ) = LAExpMinus
+let ( *. ) = LAExpMult
+
+type lBExp =
+  | LBExpLitt: bool -> lBExp
+  | LBExpNot : lBExp -> lBExp
+  | LBExpAnd : lBExp -> lBExp -> lBExp
+  | LBExpOr  : lBExp -> lBExp -> lBExp
+  | LBExpEq  : lAExp -> lAExp -> lBExp
+  | LBExpLe  : lAExp -> lAExp -> lBExp
+
+let ( !.  ) = LBExpNot
+let ( &&. ) = LBExpAnd
+let ( ||. ) = LBExpOr
+let ( ==. ) = LBExpEq
+let ( <=. ) = LBExpLe
+
+(* Class for lifting bools and ints into our language *)
+class litteral_lift a b = { v : a -> b }
+instance _ : litteral_lift int    lAExp = { v = LAExpLitt }
+instance _ : litteral_lift bool lBExp = { v = LBExpLitt }
+
+let ( !! ) = LAExpVar
+
+type lInstr =
+  | LInstrAssign : string -> lAExp -> lInstr
+  | LInstrSkip   : lInstr
+  | LInstrSeq    : lInstr -> lInstr -> lInstr
+  | LInstrIf     : lBExp -> lInstr -> lInstr -> lInstr
+  | LInstrWhile  : lBExp -> lInstr -> lInstr
+
+let ( =. ) = LInstrAssign
+let Skip = LInstrSkip
+let ( >> ) = LInstrSeq 
+
+type thenTag = | Then
+type elseTag = | Else
+type endTag  = | End
+type doTag   = | Do
+
+let iF (cond:lBExp) (_:thenTag) (b1:lInstr) (_:elseTag) (b2:lInstr) (_:endTag) : lInstr = LInstrIf cond b1 b2
+
+val while : lBExp -> doTag -> lInstr -> endTag -> lInstr
+let while cond _ body _ = LInstrWhile cond body
+
+let rec bexp_count_not (e:lBExp): nat = match e with
+  | LBExpNot (LBExpEq _ _) -> 0
+  | LBExpNot x -> 1 + bexp_count_not x
+  | LBExpAnd x y -> bexp_count_not x + bexp_count_not y
+  | LBExpOr x y -> bexp_count_not x + bexp_count_not y
+  | _ -> 0
