ToyLanguageInterpreter.fst
@@ -1,0 +1,87 @@
+module ToyLanguageInterpreter
+
+open ToyLanguageDef
+open DefaultValue
+
+open FStar.Mul
+open FStar.Tactics.Typeclasses
+
+let a = "a"
+let b = "b"
+let c = "c"
+let d = "d"
+let i = "i"
+let tmp = "tmp"
+
+let fib (max:int) =
+  (a =. (v 1)) >>
+  (b =. (v 1)) >>
+  (i =. (v 0)) >>
+  (while (!! i <=. (LAExpLitt max)) Do (
+    (tmp =. (!! a)) >>
+    (a =. (!! b)) >>
+    (b =. (!! tmp) +. (!! b)) >>
+    (i =. (!! i) +. (v 1))
+  ) End)
+
+
+type state (a:Type) = string -> a
+
+let emptyState #a [| hasDefaultValue a |] () : state a =
+  fun _ -> def
+
+val norm_lAExp : state int -> lAExp -> int
+let rec norm_lAExp state exp =
+  let fA a b g = g (norm_lAExp state a) (norm_lAExp state b) in
+  match exp with 
+  | LAExpLitt v -> v
+  | LAExpMinus a b -> fA a b ( fun x y -> x - y )
+  | LAExpMult a b -> fA a b  ( * )
+  | LAExpPlus a b -> fA a b  ( + )
+  | LAExpVar v -> state v
+
+val norm_lBExp : state int -> lBExp -> bool
+let rec norm_lBExp state exp =
+  let fA a b g = g (norm_lAExp state a) (norm_lAExp state b) in
+  let fB a b g = g (norm_lBExp state a) (norm_lBExp state b) in
+  match exp with
+  | LBExpLitt v -> v
+  | LBExpEq a b -> fA a b ( fun a b -> a = b )
+  | LBExpLe a b -> fA a b (<=)
+  | LBExpAnd a b-> fB a b (&&)
+  | LBExpOr a b -> fB a b ( || )
+  | LBExpNot a -> norm_lBExp state a
+
+class run_c a b = {
+  run : state int -> a -> b
+}
+instance _ : run_c lAExp int = { run = norm_lAExp }
+instance _ : run_c lBExp bool = { run = norm_lBExp }
+
+val norm_lInstr : state int -> lInstr -> (fuel:nat) -> Tot (state int) (decreases fuel)
+let rec norm_lInstr state instr n = if n = 0 then state else
+  let f = norm_lInstr in
+  match instr with
+  | LInstrAssign name v -> (fun q -> if q = name then run state v else state q)
+  | LInstrIf cond b1 b2 -> norm_lInstr state (if run state cond then b1 else b2) (n - 1)
+  | LInstrSkip          -> state
+  | LInstrSeq a b       -> f (f state a (n - 1)) b (n - 1)
+  | LInstrWhile cond b  -> if run state cond then
+				f state (b >> (while cond Do b End)) (n - 1)
+			  else  state
+
+instance _ : run_c lInstr (state int) = { run = fun s a -> norm_lInstr s a 100 }
+
+val execFib : int -> state int
+let execFib n = (run (emptyState ()) (fib n))
+
+let xx n = execFib n "a"
+
+let test = norm_lBExp (emptyState ()) (LBExpLitt true)
+
+
+let xxx = run (emptyState ()) (v 2 +. v 3)
+
+// let main = 
+//   let i = FStar.IO.input_int () in
+//   FStar.IO.print_string (string_of_int (xx i))
