ZeroOrLess.fst
@@ -1,0 +1,5 @@
+module ZeroOrLess
+
+open FStar.Tactics.Typeclasses
+
+class hasZeroOrLess a = {zeroOrLess: a}
